More minor simplification.  Whole development checks.  I may have introduced svn conflicts.

theories/common/certiClasses.v
@@ -104,17 +104,6 @@ Definition obsPreserving
     -> (s ⇓ sv)
     -> ∃ (dv: DstValue), (translate Src Dst s) ⇓ (Ret dv) ∧ sv ⊑ dv.
 End obsPreserving.
-(****
-Definition obsPreserving 
-  `{CerticoqTranslation Src Dst} 
-   `{BigStepOpSem Src SrcValue} `{BigStepOpSem Dst DstValue} `{GoodTerm Src}
-  :=
-   ∀ (s:Src) (sv: SrcValue), 
-    goodTerm s 
-    -> (s ⇓ sv)
-    -> forall (dv: DstValue), (translate Src Dst s) ⇓ (Ret dv) -> sv ⊑ dv.
-End obsPreserving.
-***)
 
 (* 
 Notation "s =⊏  t" := (obsLe StrongObservation s t) (at level 65). 
@@ -127,12 +116,6 @@ Arguments CerticoqLanguage2 Term Value {H} {H0} {H1} {H2}.
 Arguments obsPreserving Src Dst {H} {SrcValue} {H0} {DstValue} {H1} {H2} {H3} {H4} {H5} {H6}.
 *)
 
-(***** needed ?? **)
-Instance BigStepOpWEnv
-         (Term:Set) (ev:(environ Term) -> Term -> Term -> Prop) :
-  BigStepOpSem (Program Term) (Program Term) :=
-  λ p1 p2, ev (env p1) (main p1) (main p2) /\ (env p1 = env p2).
-(**************)
 
 Definition normalizes `{BigStepOpSem Term Value} (s:Term): Prop :=
   ∃ (sv : Value) , s ⇓ sv.
